---
title: "simplified bam"
author: "Mark Hagemann"
date: "5/6/2019"
output: html_document
---

```{r setup, include=FALSE}
knitr::opts_chunk$set(echo = TRUE)
```

This is a formal derivation of work I did in the 20181207 notebook. 

We can simplify BAM considerably as follows:

Let:

- $q = \log Q$
- $\dot{q} = q - \bar{q}$
- $x = -2/3 \log W + 1/2 \log S$
- $a = \log (A_0 + A')$
- $\tilde{n} = \log n$ (Manning's n)

Mass-conserved Manning's equation is then:

$$
q_t = -\tilde{n} + x_{st} + 5/3 a_{st}, s = 1, \dots, N_s
$$

Taking the spatial average gives:

$$
q_t = \bar{x}_{\cdot t} - \tilde{n} + \frac{5}{3} \bar{a}_{\cdot t} 
$$

Plugging this in to the first equation simplifies to: 

$$
x_{st} - \bar{x}_{\cdot t}  = - \frac{5}{3} (a_{st} - \bar{a}_{\cdot t}) 
$$

Next, assume that equation 1 only holds with an additional error term $\epsilon \sim N(0, \sigma)$. Assuming $\epsilon$ to be spatially independent makes error in equation 3 come have variance equal to $\sigma^2_* = \frac{N_s + 1}{N_s} \sigma^2$


### AMHG

The equivalent math for AMHG is

$$
w_{st} - w_c = b_s (q_t - q_c)
$$

Subtracting the spatial mean gives

$$
\bar{w}_{\cdot t} - w_c = \bar{b}(q_t - q_c)
$$

Substituting gives

$$
w_{st} - \bar{w}_{\cdot t} = (b_s - \bar{b})(q_t - q_c)
$$

Not helpful.

So the simplified method only works for Manning, and only for bathymetry. Make a stan file. 
